src/Experiments/NewPipeline/AbstractInterpretationProofs.v
@@ -18,6 +18,7 @@ Require Import Crypto.Util.Tactics.SplitInContext.
 Require Import Crypto.Util.Tactics.UniquePose.
 Require Import Crypto.Util.Tactics.SpecializeBy.
 Require Import Crypto.Util.Tactics.SpecializeAllWays.
+Require Import Crypto.Util.Tactics.Head.
 Require Import Crypto.Experiments.NewPipeline.Language.
 Require Import Crypto.Experiments.NewPipeline.LanguageInversion.
 Require Import Crypto.Experiments.NewPipeline.LanguageWf.
@@ -45,19 +46,147 @@ Module Compilers.
       Let type_base (x : base_type) : type := type.base x.
       Local Coercion type_base : base_type >-> type.
       Context {ident : type -> Type}.
-      Local Notation expr := (@expr base_type ident).
       Local Notation Expr := (@expr.Expr base_type ident).
-      Local Notation UnderLets := (@UnderLets base_type ident).
-      Context (abstract_domain' : base_type -> Type)
+      Context (abstract_domain' base_interp : base_type -> Type)
+              (abstraction_relation' : forall t, abstract_domain' t -> base_interp t -> Prop)
               (bottom' : forall A, abstract_domain' A)
+              (bottom'_related : forall t v, abstraction_relation' t (bottom' t) v)
               (abstract_interp_ident : forall t, ident t -> type.interp abstract_domain' t)
-              (abstract_domain'_R : forall t, abstract_domain' t -> abstract_domain' t -> Prop)
-              {abstract_interp_ident_Proper : forall t, Proper (eq ==> abstract_domain'_R t) (abstract_interp_ident t)}
-              {bottom'_Proper : forall t, Proper (abstract_domain'_R t) (bottom' t)}.
+              (interp_ident : forall t, ident t -> type.interp base_interp t)
+              (interp_ident_Proper : forall t (idc : ident t), type.related_hetero abstraction_relation' (abstract_interp_ident t idc) (interp_ident t idc)).
       Local Notation abstract_domain := (@abstract_domain base_type abstract_domain').
+      Definition abstraction_relation {t} : abstract_domain t -> type.interp base_interp t -> Prop
+        := type.related_hetero (@abstraction_relation').
       Local Notation bottom := (@bottom base_type abstract_domain' (@bottom')).
       Local Notation bottom_for_each_lhs_of_arrow := (@bottom_for_each_lhs_of_arrow base_type abstract_domain' (@bottom')).
-      Local Notation abstract_domain_R := (@abstract_domain_R base_type abstract_domain' abstract_domain'_R).
+      Local Notation var := (type.interp base_interp).
+      Local Notation expr := (@expr base_type ident var).
+      Local Notation UnderLets := (@UnderLets base_type ident var).
+      Local Notation value := (@value base_type ident var abstract_domain').
+      Local Notation value_with_lets := (@value_with_lets base_type ident var abstract_domain').
+      Local Notation state_of_value := (@state_of_value base_type ident var abstract_domain').
+      Context (annotate : forall (is_let_bound : bool) t, abstract_domain' t -> expr t -> UnderLets (expr t)).
+      (*
+      Local Notation reify1 := (@reify base_type ident var1 abstract_domain' annotate1 bottom').
+      Local Notation reify2 := (@reify base_type ident var2 abstract_domain' annotate2 bottom').
+      Local Notation reflect1 := (@reflect base_type ident var1 abstract_domain' annotate1 bottom').
+      Local Notation reflect2 := (@reflect base_type ident var2 abstract_domain' annotate2 bottom').
+      Local Notation interp1 := (@interp base_type ident var1 abstract_domain' annotate1 bottom' interp_ident1).
+      Local Notation interp2 := (@interp base_type ident var2 abstract_domain' annotate2 bottom' interp_ident2).
+      Local Notation eval_with_bound'1 := (@eval_with_bound' base_type ident var1 abstract_domain' annotate1 bottom' interp_ident1).
+      Local Notation eval_with_bound'2 := (@eval_with_bound' base_type ident var2 abstract_domain' annotate2 bottom' interp_ident2).
+      Local Notation eval'1 := (@eval' base_type ident var1 abstract_domain' annotate1 bottom' interp_ident1).
+      Local Notation eval'2 := (@eval' base_type ident var2 abstract_domain' annotate2 bottom' interp_ident2).
+      Local Notation eta_expand_with_bound'1 := (@eta_expand_with_bound' base_type ident var1 abstract_domain' annotate1 bottom').
+      Local Notation eta_expand_with_bound'2 := (@eta_expand_with_bound' base_type ident var2 abstract_domain' annotate2 bottom').
+*)
+(*
+
+      Fixpoint value (t : type)
+        := (abstract_domain t
+            * match t return Type (* COQBUG(https://github.com/coq/coq/issues/7727) *) with
+              | type.base t
+                => @expr var t
+              | type.arrow s d
+                => value s -> UnderLets (value d)
+              end)%type.
+
+      Definition value_with_lets (t : type)
+        := UnderLets (value t).
+
+
+      Fixpoint bottom {t} : abstract_domain t
+        := match t with
+           | type.base t => bottom' t
+           | type.arrow s d => fun _ => @bottom d
+           end.
+
+      Fixpoint bottom_for_each_lhs_of_arrow {t} : type.for_each_lhs_of_arrow abstract_domain t
+        := match t return type.for_each_lhs_of_arrow abstract_domain t with
+           | type.base t => tt
+           | type.arrow s d => (bottom, @bottom_for_each_lhs_of_arrow d)
+           end.
+
+      Definition state_of_value {t} : value t -> abstract_domain t
+        := match t return value t -> abstract_domain t with
+           | type.base t => fun '(st, v) => st
+           | type.arrow s d => fun '(st, v) => st
+           end.
+
+      Fixpoint reify (is_let_bound : bool) {t} : value t -> type.for_each_lhs_of_arrow abstract_domain t -> UnderLets (@expr var t)
+        := match t return value t -> type.for_each_lhs_of_arrow abstract_domain t -> UnderLets (@expr var t) with
+           | type.base t
+             => fun '(st, v) 'tt
+                => annotate is_let_bound t st v
+           | type.arrow s d
+             => fun '(f_st, f_e) '(sv, dv)
+                => Base
+                     (λ x , (UnderLets.to_expr
+                               (fx <-- f_e (@reflect _ (expr.Var x) sv);
+                                  @reify false _ fx dv)))
+           end%core%expr
+      with reflect {t} : @expr var t -> abstract_domain t -> value t
+           := match t return @expr var t -> abstract_domain t -> value t with
+              | type.base t
+                => fun e st => (st, e)
+              | type.arrow s d
+                => fun e absf
+                   => (absf,
+                       (fun v
+                        => let stv := state_of_value v in
+                           (rv <-- (@reify false s v bottom_for_each_lhs_of_arrow);
+                              Base (@reflect d (e @ rv) (absf stv))%expr)))
+              end%under_lets.
+
+      (* N.B. Because the [App] case only looks at the second argument
+              of arrow-values, we are free to set the state of [Abs]
+              nodes to [bottom], because for any [Abs] nodes which are
+              actually applied (here and in places where we don't
+              rewrite), we just drop it. *)
+      Fixpoint interp {t} (e : @expr value_with_lets t) : value_with_lets t
+        := match e in expr.expr t return value_with_lets t with
+           | expr.Ident t idc => interp_ident _ idc (* Base (reflect (###idc) (abstract_interp_ident _ idc))*)
+           | expr.Var t v => v
+           | expr.Abs s d f => Base (bottom, fun x => @interp d (f (Base x)))
+           | expr.App s d f x
+             => (x' <-- @interp s x;
+                   f' <-- @interp (s -> d)%etype f;
+                   snd f' x')
+           | expr.LetIn (type.arrow _ _) B x f
+             => (x' <-- @interp _ x;
+                   @interp _ (f (Base x')))
+           | expr.LetIn (type.base A) B x f
+             => (x' <-- @interp _ x;
+                   x'' <-- reify true (* this forces a let-binder here *) x' tt;
+                   @interp _ (f (Base (reflect x'' (state_of_value x')))))
+           end%under_lets.
+
+      Definition eval_with_bound' {t} (e : @expr value_with_lets t)
+                 (st : type.for_each_lhs_of_arrow abstract_domain t)
+        : expr t
+        := UnderLets.to_expr (e' <-- interp e; reify false e' st).
+
+      Definition eval' {t} (e : @expr value_with_lets t) : expr t
+        := eval_with_bound' e bottom_for_each_lhs_of_arrow.
+
+      Definition eta_expand_with_bound' {t} (e : @expr var t)
+                 (st : type.for_each_lhs_of_arrow abstract_domain t)
+        : expr t
+        := UnderLets.to_expr (reify false (reflect e bottom) st).
+
+      Section extract.
+        Context (ident_extract : forall t, ident t -> abstract_domain t).
+
+        Definition extract' {t} (e : @expr abstract_domain t) : abstract_domain t
+          := expr.interp (@ident_extract) e.
+
+        Definition extract_gen {t} (e : @expr abstract_domain t) (bound : type.for_each_lhs_of_arrow abstract_domain t)
+          : abstract_domain' (type.final_codomain t)
+          := type.app_curried (extract' e) bound.
+      End extract.
+    End with_var.
+
+
 
       Section extract.
         Context (ident_extract : forall t, ident t -> abstract_domain t)
@@ -82,8 +211,9 @@ Module Compilers.
           eapply extract'_Proper; eassumption.
         Qed.
       End extract.
+*)
     End with_type.
-
+(*
     Module ident.
       Import defaults.
       Local Notation UnderLets := (@UnderLets base.type ident).
@@ -118,7 +248,7 @@ Module Compilers.
         End extract.
       End with_type.
     End ident.
-
+*)
     Section specialized.
       Import defaults.
       Local Notation abstract_domain' := ZRange.type.base.option.interp (only parsing).
@@ -201,58 +331,91 @@ Module Compilers.
   End partial.
   Import defaults.
 
+  Module Import CheckCasts.
+    Module ident.
+      Lemma interp_eqv_without_casts t idc
+            cast_outside_of_range1 cast_outside_of_range2
+            (Hc : partial.is_annotation t idc = false)
+      : ident.gen_interp cast_outside_of_range1 idc
+        == ident.gen_interp cast_outside_of_range2 idc.
+      Proof.
+        generalize (@ident.gen_interp_Proper cast_outside_of_range1 t idc idc eq_refl);
+          destruct idc; try exact id; cbn in Hc; discriminate.
+      Qed.
+    End ident.
+
+    Lemma interp_eqv_without_casts
+          cast_outside_of_range1 cast_outside_of_range2
+          G {t} e1 e2 e3
+          (HG : forall t v1 v2 v3, List.In (existT _ t (v1, v2, v3)) G -> v2 == v3)
+          (Hwf : expr.wf3 G e1 e2 e3)
+          (Hc : @CheckCasts.get_casts t e1 = nil)
+    : expr.interp (@ident.gen_interp cast_outside_of_range1) e2
+      == expr.interp (@ident.gen_interp cast_outside_of_range2) e3.
+    Proof.
+      induction Hwf;
+        repeat first [ progress cbn [CheckCasts.get_casts] in *
+                     | discriminate
+                     | match goal with
+                       | [ H : (_ ++ _)%list = nil |- _ ] => apply List.app_eq_nil in H
+                       end
+                     | progress destruct_head'_and
+                     | progress break_innermost_match_hyps
+                     | progress interp_safe_t
+                     | solve [ eauto using ident.interp_eqv_without_casts ] ].
+    Qed.
+
+    Lemma Interp_WithoutUnsupportedCasts {t} (e : Expr t)
+          (Hc : CheckCasts.GetUnsupportedCasts e = nil)
+          (Hwf : expr.Wf3 e)
+          cast_outside_of_range1 cast_outside_of_range2
+      : expr.Interp (@ident.gen_interp cast_outside_of_range1) e
+        == expr.Interp (@ident.gen_interp cast_outside_of_range2) e.
+    Proof. eapply interp_eqv_without_casts with (G:=nil); wf_safe_t. Qed.
+  End CheckCasts.
+
   Module RelaxZRange.
+    Definition relaxed_cast_outside_of_range
+               (relax_zrange : zrange -> option zrange)
+               (cast_outside_of_range : zrange -> Z -> Z)
+    : zrange -> Z -> Z
+      := fun r v
+         => match relax_zrange r with
+            | Some r' => ident.cast cast_outside_of_range r' v
+            | None => cast_outside_of_range r v
+            end.
+
     Module ident.
       Section relax.
         Context (relax_zrange : zrange -> option zrange)
+                (cast_outside_of_range : zrange -> Z -> Z)
                 (Hrelax : forall r r' z, is_tighter_than_bool z r = true
                                          -> relax_zrange r = Some r'
                                          -> is_tighter_than_bool z r' = true).
 
-        Lemma interp_relax {t} (idc idc' : ident t)
-              (Hidc : @RelaxZRange.ident.relax relax_zrange t idc = Some idc')
-              v
-              (Hinterp : forall cast_outside_of_range, type.app_curried (ident.gen_interp cast_outside_of_range idc) v = type.app_curried (ident.interp idc) v)
-          : forall cast_outside_of_range, type.app_curried (ident.gen_interp cast_outside_of_range idc') v = type.app_curried (ident.interp idc) v.
+        Local Notation relaxed_cast_outside_of_range := (@relaxed_cast_outside_of_range relax_zrange cast_outside_of_range).
+
+        Lemma interp_relax {t} (idc : ident t)
+          : ident.gen_interp cast_outside_of_range (@RelaxZRange.ident.relax relax_zrange t idc)
+            == ident.gen_interp relaxed_cast_outside_of_range idc.
         Proof.
-          intro cast_outside_of_range.
-          pose proof (Hinterp (fun _ => id)).
-          pose proof (fun myrange => Hinterp (fun _ => cast_outside_of_range myrange)).
-          destruct idc; cbv [RelaxZRange.ident.relax Option.bind] in *; inversion_option; break_innermost_match_hyps; inversion_option; subst;
-            repeat match goal with
-                   | [ H : relax_zrange _ = Some _ |- _ ] => unique pose proof (fun zl zu pf => Hrelax _ _ (Build_zrange zl zu) pf H)
-                   end;
-            repeat first [ reflexivity
+          pose proof (@ident.gen_interp_Proper cast_outside_of_range t idc idc eq_refl) as Hp.
+          destruct idc; cbn [type.related] in *; repeat (let x := fresh "x" in intro x; specialize (Hp x));
+            repeat first [ assumption
+                         | reflexivity
                          | discriminate
                          | congruence
-                         | progress cbv [RelaxZRange.ident.relax Option.bind id ident.cast is_tighter_than_bool] in *
-                         | progress cbn [fst snd] in *
                          | progress subst
-                         | progress inversion_option
-                         | progress inversion_prod
+                         | progress cbv [relaxed_cast_outside_of_range RelaxZRange.ident.relax Option.bind ident.cast respectful is_tighter_than_bool id] in *
+                         | progress cbn [ident.gen_interp type.related type.interp base.interp upper lower] in *
                          | progress destruct_head'_prod
-                         | progress destruct_head'_and
-                         | progress cbn in *
-                         | progress Bool.split_andb
-                         | progress intros
+                         | progress specialize_by (exact eq_refl)
+                         | break_match_step ltac:(fun x => let h := head x in constr_eq h relax_zrange)
                          | match goal with
-                           | [ H : forall x, (_, _) = (_, _) |- _ ]
-                             => pose proof (fun x => f_equal (@fst _ _) (H x));
-                               pose proof (fun x => f_equal (@snd _ _) (H x));
-                               clear H
-                           | [ H : context[andb _ _ = true] |- _ ] => rewrite Bool.andb_true_iff in H || setoid_rewrite Bool.andb_true_iff in H
-                           | [ H : context[Z.leb _ _ = true] |- _ ] => rewrite Z.leb_le in H || setoid_rewrite Z.leb_le in H
-                           | [ H : forall a b, and (Z.le ?x a) (Z.le b ?y) -> _ /\ _, H' : Z.le ?x _, H'' : Z.le _ ?y |- _ ]
-                             => unique pose proof (proj1 (H _ _ (conj H' H'')));
-                                unique pose proof (proj2 (H _ _ (conj H' H'')))
+                           | [ H : relax_zrange ?r = Some ?r' |- context[Z.leb (lower ?r) ?v] ]
+                             => pose proof (fun pf => Hrelax _ _ (Build_zrange v v) pf H); clear H
                            end
-                         | progress rewrite ?Bool.andb_false_iff in *
-                         | progress destruct_head'_or
-                         | progress break_innermost_match_hyps
-                         | progress break_innermost_match
-                         | progress Z.ltb_to_lt
-                         | apply (f_equal2 (@pair _ _))
-                         | lia ].
+                         | break_innermost_match_step ].
         Qed.
       End relax.
     End ident.
@@ -262,63 +425,27 @@ Module Compilers.
         Context (relax_zrange : zrange -> option zrange)
                 (Hrelax : forall r r' z, is_tighter_than_bool z r = true
                                          -> relax_zrange r = Some r'
-                                         -> is_tighter_than_bool z r' = true).
-        Lemma interp_relax {t} (e : expr t)
-              v
-              (Hinterp : forall cast_outside_of_range, type.app_curried (expr.interp (@ident.gen_interp cast_outside_of_range) e) v
-                                                  = type.app_curried (defaults.interp e) v)
-          : forall cast_outside_of_range, type.app_curried (expr.interp (@ident.gen_interp cast_outside_of_range) (RelaxZRange.expr.relax relax_zrange e)) v
-                                     = type.app_curried (defaults.interp e) v.
+                                         -> is_tighter_than_bool z r' = true)
+                (cast_outside_of_range : zrange -> Z -> Z).
+
+        Local Notation relaxed_cast_outside_of_range := (@relaxed_cast_outside_of_range relax_zrange cast_outside_of_range).
+
+        Lemma interp_relax G {t} (e1 e2 : expr t)
+              (HG : forall t v1 v2, List.In (existT _ t (v1, v2)) G -> v1 == v2)
+              (Hwf : expr.wf G e1 e2)
+          : expr.interp (@ident.gen_interp cast_outside_of_range) (RelaxZRange.expr.relax relax_zrange e1)
+            == expr.interp (@ident.gen_interp relaxed_cast_outside_of_range) e2.
         Proof.
-          intro cast_outside_of_range; rewrite <- (Hinterp cast_outside_of_range); pose proof (Hinterp cast_outside_of_range).
-          induction e; cbn -[RelaxZRange.ident.relax] in *; interp_safe_t; cbv [option_map] in *;
+          induction Hwf; cbn -[RelaxZRange.ident.relax] in *; interp_safe_t; cbv [option_map] in *;
             break_innermost_match; cbn -[RelaxZRange.ident.relax] in *; interp_safe_t;
-              eauto using tt.
-          all: repeat first [ reflexivity
-                            | progress intros
-                            | progress specialize_by_assumption
-                            | progress cbn -[RelaxZRange.ident.relax] in *
-                            | match goal with
-                              | [ H : unit -> ?T |- _ ] => specialize (H tt)
-                              | [ H : forall x : _ * _, _ |- _ ] => specialize (fun a b => H (a, b))
-                              | [ e : expr (type.base (base.type.type_base base.type.unit)) |- _ ]
-                                => match goal with
-                                  | [ |- context[expr.interp ?ii e] ] => destruct (expr.interp ii e)
-                                  | [ H : context[expr.interp ?ii e] |- _ ] => destruct (expr.interp ii e)
-                                  end
-                              end
-                            | progress cbn [fst snd] in *
-                            | match goal with
-                              | [ H : _ |- _ ] => rewrite H
-                              end ].
-          all: specialize_all_ways.
-          all: repeat first [ reflexivity
-                            | progress intros
-                            | progress specialize_by_assumption
-                            | progress cbn -[RelaxZRange.ident.relax] in *
-                            | match goal with
-                              | [ H : unit -> ?T |- _ ] => specialize (H tt)
-                              | [ H : forall x : _ * _, _ |- _ ] => specialize (fun a b => H (a, b))
-                              | [ e : expr (type.base (base.type.type_base base.type.unit)) |- _ ]
-                                => match goal with
-                                  | [ |- context[expr.interp ?ii e] ] => destruct (expr.interp ii e)
-                                  | [ H : context[expr.interp ?ii e] |- _ ] => destruct (expr.interp ii e)
-                                  end
-                              end
-                            | progress cbn [fst snd] in *
-                            | match goal with
-                              | [ H : _ |- _ ] => rewrite H
-                              end ].
-        Admitted.
+              eauto using tt, @ident.interp_relax.
+        Qed.
 
         Lemma Interp_Relax {t} (e : Expr t)
-              (Hwf : expr.Wf3 e)
-              v
-              (Hinterp : forall cast_outside_of_range, type.app_curried (expr.Interp (@ident.gen_interp cast_outside_of_range) e) v
-                                                  = type.app_curried (defaults.Interp e) v)
-          : forall cast_outside_of_range, type.app_curried (expr.Interp (@ident.gen_interp cast_outside_of_range) (RelaxZRange.expr.Relax relax_zrange e)) v
-                                     = type.app_curried (defaults.Interp e) v.
-        Proof. eapply @interp_relax; try assumption. Qed.
+              (Hwf : Wf e)
+          : expr.Interp (@ident.gen_interp cast_outside_of_range) (RelaxZRange.expr.Relax relax_zrange e)
+            == expr.Interp (@ident.gen_interp relaxed_cast_outside_of_range) e.
+        Proof. apply interp_relax with (G:=nil); wf_safe_t. Qed.
       End relax.
     End expr.
   End RelaxZRange.
@@ -336,11 +463,12 @@ Module Compilers.
         (Harg12 : type.and_for_each_lhs_of_arrow (@type.eqv) arg1 arg2)
         (Harg1 : type.andb_bool_for_each_lhs_of_arrow (@ZRange.type.option.is_bounded_by) b_in arg1 = true),
       type.app_curried (expr.Interp (@ident.gen_interp cast_outside_of_range) (PartialEvaluateWithBounds E b_in)) arg1
-      = type.app_curried (Interp E) arg2.
+      = type.app_curried (expr.Interp (@ident.gen_interp cast_outside_of_range) E) arg2.
   Proof.
   Admitted.
 
   Lemma Interp_PartialEvaluateWithBounds_bounded
+        cast_outside_of_range
         {t} (E : Expr t)
         (Hwf : Wf E)
         (b_in : type.for_each_lhs_of_arrow ZRange.type.option.interp t)
@@ -348,7 +476,7 @@ Module Compilers.
         (Harg1 : type.andb_bool_for_each_lhs_of_arrow (@ZRange.type.option.is_bounded_by) b_in arg1 = true),
       ZRange.type.base.option.is_bounded_by
         (partial.Extract (PartialEvaluateWithBounds E b_in) b_in)
-        (type.app_curried (expr.Interp (@ident.interp) (PartialEvaluateWithBounds E b_in)) arg1)
+        (type.app_curried (expr.Interp (@ident.gen_interp cast_outside_of_range) (PartialEvaluateWithBounds E b_in)) arg1)
       = true.
   Proof.
   Admitted.
@@ -362,6 +490,7 @@ Module Compilers.
         (Harg1 : type.andb_bool_for_each_lhs_of_arrow (@ZRange.type.option.is_bounded_by) b_in arg1 = true),
       type.app_curried (Interp (PartialEvaluateWithListInfoFromBounds E b_in)) arg1 = type.app_curried (Interp E) arg2.
   Proof.
+    cbv [PartialEvaluateWithListInfoFromBounds].
   Admitted.
 
   Theorem CheckedPartialEvaluateWithBounds_Correct
@@ -385,6 +514,14 @@ Module Compilers.
   Proof.
     cbv [CheckedPartialEvaluateWithBounds CheckPartialEvaluateWithBounds Let_In] in *;
       break_innermost_match_hyps; inversion_sum; subst.
+    let H := lazymatch goal with H : _ = nil |- _ => H end in
+    pose proof (@Interp_WithoutUnsupportedCasts _ _ H ltac:(solve [ auto with wf ])) as H'; clear H;
+      assert (forall cast_outside_of_range1 cast_outside_of_range2,
+                 expr.Interp (@ident.gen_interp cast_outside_of_range1) E == expr.Interp (@ident.gen_interp cast_outside_of_range2) E)
+      by (intros c1 c2; specialize (H' c1 c2);
+          rewrite !@GeneralizeVar.Interp_gen1_FromFlat_ToFlat in H' by eauto with wf typeclass_instances;
+          assumption).
+    clear H'.
     split.
     { intros arg1 arg2 Harg12 Harg1.
       assert (arg1_Proper : Proper (type.and_for_each_lhs_of_arrow (@type.related base.type base.interp (fun _ => eq))) arg1)
@@ -398,6 +535,8 @@ Module Compilers.
                         | rewrite RelaxZRange.expr.Interp_Relax; eauto
                         | erewrite !Interp_PartialEvaluateWithBounds
                         | solve [ eauto with wf ]
+                        | apply type.app_curried_Proper
+                        | apply expr.Wf_Interp_Proper_gen
                         | progress intros ]. }
     { auto with wf. }
   Qed.
